pool and unpool entrypoints for pooled consistency in the metaspecification

specifications/StructuredPoolsSpec/StructuredPoolsSpec.v
@@ -12,6 +12,7 @@ From ConCert.Utils Require Import RecordUpdate.
 From ConCert.Utils Require Import Extras.
 From Coq Require Import FunctionalExtensionality.
 From Coq Require Import Ensembles.
+From Coq Require Import Permutation.
 From Coq Require Import ZArith_base.
 From Coq Require Import QArith_base.
 From Coq Require Import String.
@@ -145,12 +146,16 @@ Class Msg_Spec (T : Type) :=
     - number of outstanding pool tokens
 *)
 Class State_Spec (T : Type) := 
-  build_state_spec {
-    stor_rates : T -> FMap token exchange_rate ;
-    stor_tokens_held : T -> FMap token N ;
-    stor_pool_token : T -> token ; 
-    stor_outstanding_tokens : T -> N ;
-}.
+    build_state_spec {
+      (* the exchange rates *)
+      stor_rates : T -> FMap token exchange_rate ;
+      (* token balances *)
+      stor_tokens_held : T -> FMap token N ;
+      (* pool token data *)
+      stor_pool_token : T -> token ; 
+      (* number of outstanding pool tokens *)
+      stor_outstanding_tokens : T -> N ;
+  }.
 
 (* specification of the Setup type 
   to initialize the contract, we need:
@@ -181,138 +186,94 @@ Definition none_fails (contract : Contract Setup Msg State Error) : Prop :=
     receive contract chain ctx cstate None = Err err.
 
 (* Specification of the POOL entrypoint *)
-(* When the POOL entrypoint is called, the contract call fails if 
-    the token to be pooled is not in the family of semi-fungible tokens. *)
+(* A call to the DEPOSIT entrypoint fails if the token to be pooled is not in the 
+    rates map held in the storage (=> is not in T) *)
 Definition pool_entrypoint_check (contract : Contract Setup Msg State Error) : Prop :=
-    forall bstate caddr cstate chain ctx msg msg_payload,
-    (* reachable bstate *)
-    reachable bstate -> 
-    (* the contract address is caddr with state cstate *)
-    env_contracts bstate caddr = Some (contract : WeakContract) -> 
-    contract_state bstate caddr = Some cstate -> 
-    (* forall calls to the Pool entrypoint *)
-    msg = pool (msg_payload) -> 
-    (* the receive function returns an error if the token to be pooled is not in the 
-       rates map held in the storage (=> is not in the semi-fungible family) *)
+    forall cstate chain ctx msg_payload,
+    (* If there is no entry in the rates map for the token to be pooled, *)
     FMap.find msg_payload.(token_pooled) (stor_rates cstate) = None -> 
-    receive contract chain ctx cstate (Some msg) = 
+    (* the transaction fails. *)
+    receive contract chain ctx cstate (Some (pool (msg_payload))) = 
       Err(error_to_Error error_TOKEN_NOT_FOUND).
 
-
+(* A successful call to DEPOSIT means that token_pooled has an exchange rate (=> is in T) *)
 Definition pool_entrypoint_check_2 (contract : Contract Setup Msg State Error) : Prop :=
-    forall bstate caddr cstate cstate' chain ctx msg msg_payload acts,
-    (* reachable bstate *)
-    reachable bstate -> 
-    (* the contract address is caddr with state cstate *)
-    env_contracts bstate caddr = Some (contract : WeakContract) -> 
-    contract_state bstate caddr = Some cstate -> 
-    (* forall calls to the Pool entrypoint *)
-    msg = pool (msg_payload) -> 
-    (* the receive function returns an error if the token to be pooled is not in the 
-       rates map held in the storage (=> is not in the semi-fungible family) *)
-    receive contract chain ctx cstate (Some msg) = Ok(cstate', acts) -> 
+    forall cstate cstate' chain ctx msg_payload acts,
+    (* a successful call *)
+    receive contract chain ctx cstate (Some (pool (msg_payload))) = Ok(cstate', acts) -> 
+    (* an exchange rate exists *)
     exists r_x, 
     FMap.find msg_payload.(token_pooled) (stor_rates cstate) = Some r_x.
 
-
-(* When the POOL entrypoint is successfully called, it emits a TRANSFER call to the 
+(* When the DEPOSIT entrypoint is successfully called, it emits a TRANSFER call to the 
     token in storage, with q tokens in the payload of the call *)
-Definition pool_emits_transfer (contract : Contract Setup Msg State Error) : Prop := 
-    forall bstate caddr cstate chain ctx msg msg_payload cstate' acts,
-    (* reachable bstate *)
-    reachable bstate -> 
-    (* the contract address is caddr with state cstate *)
-    env_contracts bstate caddr = Some (contract : WeakContract) -> 
-    contract_state bstate caddr = Some cstate -> 
-    (* the call to POOL was successful *)
-    msg = pool (msg_payload) -> 
-    receive contract chain ctx cstate (Some msg) = Ok(cstate', acts) -> 
+Definition pool_emits_txns (contract : Contract Setup Msg State Error) : Prop := 
+    forall cstate chain ctx msg_payload cstate' acts,
+    (* the call to DEPOSIT was successful *)
+    receive contract chain ctx cstate (Some (pool (msg_payload))) = Ok(cstate', acts) -> 
     (* in the acts list there is a transfer call with q tokens as the payload *)
-    exists transfer_to transfer_data transfer_payload,
+    exists transfer_to transfer_data transfer_payload mint_data mint_payload,
     (* there is a transfer call *)
-    In 
-    (act_call 
-        (msg_payload.(token_pooled).(FA2Spec.token_address)) (* call to the token address *)
-        0 (* with amount = 0 *)
-        (serialize (FA2Spec.Transfer transfer_payload)))
-    acts /\ 
+    let transfer_call := (act_call 
+        (* calls the pooled token address *)
+        (msg_payload.(token_pooled).(FA2Spec.token_address)) 
+        (* with amount 0 *)
+        0
+        (* and payload transfer_payload *)
+        (serialize (FA2Spec.Transfer transfer_payload))) in 
     (* with a transfer in it *)
     In transfer_data transfer_payload /\ 
     (* which itself has transfer data *)
     In transfer_to transfer_data.(FA2Spec.txs) /\
     (* whose quantity is the quantity pooled *)
-    transfer_to.(FA2Spec.amount) = msg_payload.(qty_pooled).
-
-
-(* When the POOL entrypoint is successfully called, it emits a MINT call to the 
-    pool_token, with q * r_x / 1_000_000 in the payload *)
-Definition pool_emits_mint (contract : Contract Setup Msg State Error) : Prop := 
-    forall bstate caddr cstate chain ctx msg msg_payload cstate' acts,
-    (* reachable bstate *)
-    reachable bstate -> 
-    (* the contract address is caddr with state cstate *)
-    env_contracts bstate caddr = Some (contract : WeakContract) -> 
-    contract_state bstate caddr = Some cstate -> 
-    (* the call to POOL was successful *)
-    msg = pool msg_payload -> 
-    receive contract chain ctx cstate (Some msg) = Ok(cstate', acts) -> 
-    (* in the acts list there is a MINT call with q * r_x / 1_000_000 in the payload *)
-    exists mint_data mint_payload,
+    transfer_to.(FA2Spec.amount) = msg_payload.(qty_pooled) /\
     (* there is a mint call in acts *)
-    In 
-    (act_call
-        (stor_pool_token cstate).(FA2Spec.token_address) (* calls the pool token address *)
-        0 (* with amount 0 *)
-        (serialize (FA2Spec.Mint mint_payload)))
-    acts /\ 
+    let mint_call := (act_call 
+        (* calls the pool token contract *)
+        (stor_pool_token cstate).(FA2Spec.token_address) 
+        (* with amount 0 *)
+        0 
+        (* and payload mint_payload *)
+        (serialize (FA2Spec.Mint mint_payload))) in 
     (* with has mint_data in the payload *)
     In mint_data mint_payload /\
     (* and the mint data has these properties: *)
     let r_x := get_rate msg_payload.(token_pooled) (stor_rates cstate) in 
     mint_data.(FA2Spec.qty) = msg_payload.(qty_pooled) * r_x / 1_000_000 /\
-    (* TODO perhaps also specify that the minted tokens go to pooler *)
-    mint_data.(FA2Spec.mint_owner) = ctx.(ctx_from).
+    mint_data.(FA2Spec.mint_owner) = ctx.(ctx_from) /\ 
+    (* these are the only emitted transactions *)
+    (acts = [ transfer_call ; mint_call ] \/
+    acts = [ mint_call ; transfer_call ]).
 
-(* When the POOL entrypoint is successfully called, the TRANSFER and MINT transactions
-    are the only transactions emitted by the contract *)
-Definition pool_atomic (contract : Contract Setup Msg State Error) : Prop := 
-    forall bstate caddr cstate chain ctx msg msg_payload cstate' acts, 
-    (* reachable bstate *)
-    reachable bstate -> 
-    (* the contract address is caddr with state cstate *)
-    env_contracts bstate caddr = Some (contract : WeakContract) -> 
-    contract_state bstate caddr = Some cstate -> 
-    (* the call to POOL was successful *)
-    msg = pool msg_payload -> 
-    receive contract chain ctx cstate (Some msg) = Ok(cstate', acts) -> 
-    (* we have a MINT call in acts and a TRANSFER call *)
-    length acts = 2%nat.
-
-
-(* When the POOL entrypoint is successfully called, tokens_held goes up appropriately *)
+(* When the DEPOSIT entrypoint is successfully called, tokens_held goes up appropriately *)
 Definition pool_increases_tokens_held (contract : Contract Setup Msg State Error) : Prop := 
     forall cstate chain ctx msg_payload cstate' acts,
-    (* the call to POOL was successful *)
+    (* the call to DEPOSIT was successful *)
     receive contract chain ctx cstate (Some (pool msg_payload)) = Ok(cstate', acts) -> 
     (* in cstate', tokens_held has increased at token *)
     let token := msg_payload.(token_pooled) in
     let qty := msg_payload.(qty_pooled) in
     let old_bal := get_bal token (stor_tokens_held cstate) in 
     let new_bal := get_bal token (stor_tokens_held cstate') in 
-    new_bal = old_bal + qty.
+    new_bal = old_bal + qty /\ 
+    forall t,
+    t <> token -> 
+    get_bal t (stor_tokens_held cstate) = 
+    get_bal t (stor_tokens_held cstate').
 
-
+(* And the rates don't change *)
 Definition pool_rates_unchanged (contract : Contract Setup Msg State Error) : Prop := 
     forall cstate cstate' chain ctx msg_payload acts,
-    (* the call to POOL was successful *)
+    (* the call to DEPOSIT was successful *)
     receive contract chain ctx cstate (Some (pool msg_payload)) = Ok(cstate', acts) -> 
     (* rates all stay the same *)
     forall t,
     FMap.find t (stor_rates cstate) = FMap.find t (stor_rates cstate').
 
+(* The outstanding tokens change appropriately *)
 Definition pool_outstanding (contract : Contract Setup Msg State Error) : Prop := 
     forall cstate cstate' chain ctx msg_payload acts,
-    (* the call to POOL was successful *)
+    (* the call to DEPOSIT was successful *)
     receive contract chain ctx cstate (Some (pool msg_payload)) = Ok(cstate', acts) -> 
     (* rates all stay the same *)
     let rate_in := get_rate msg_payload.(token_pooled) (stor_rates cstate) in 
@@ -321,115 +282,98 @@ Definition pool_outstanding (contract : Contract Setup Msg State Error) : Prop :
     stor_outstanding_tokens cstate + rate_in / 1000000 * qty.
 
 (* Specification of the UNPOOL entrypoint *)
-(* When the UNPOOL entrypoint is called, the contract call fails if 
-    the token to be pooled is not in the family of semi-fungible tokens. *)
+
+(* A call to the WITHDRAW entrypoint fails if the token to be unpooled is not in the 
+    rates map held in the storage (=> is not in T) *)
 Definition unpool_entrypoint_check (contract : Contract Setup Msg State Error) : Prop :=
-    forall bstate caddr cstate chain ctx msg msg_payload,
-    (* reachable bstate *)
-    reachable bstate -> 
-    (* the contract address is caddr with state cstate *)
-    env_contracts bstate caddr = Some (contract : WeakContract) -> 
-    contract_state bstate caddr = Some cstate -> 
-    (* forall calls to the Pool entrypoint *)
-    msg = unpool (msg_payload) -> 
-    (* the receive function returns an error if the token to be pooled is not in the 
-       rates map held in the storage (=> is not in the semi-fungible family) *)
+    forall cstate chain ctx msg_payload,
+    (* If there is no entry in the rates map for the token to be unpooled, *)
     FMap.find msg_payload.(token_unpooled) (stor_rates cstate) = None -> 
-    receive contract chain ctx cstate (Some msg) = 
+    (* the transaction fails. *)
+    receive contract chain ctx cstate (Some (unpool (msg_payload))) = 
       Err(error_to_Error error_TOKEN_NOT_FOUND).
 
 
+(* A successful call to WITHDRAW means that token_pooled has an exchange rate (=> is in T) *)
 Definition unpool_entrypoint_check_2 (contract : Contract Setup Msg State Error) : Prop :=
-    forall bstate caddr cstate cstate' chain ctx msg msg_payload acts,
-    (* reachable bstate *)
-    reachable bstate -> 
-    (* the contract address is caddr with state cstate *)
-    env_contracts bstate caddr = Some (contract : WeakContract) -> 
-    contract_state bstate caddr = Some cstate -> 
-    (* forall calls to the Pool entrypoint *)
-    msg = unpool (msg_payload) -> 
-    (* the receive function returns an error if the token to be pooled is not in the 
-       rates map held in the storage (=> is not in the semi-fungible family) *)
-    receive contract chain ctx cstate (Some msg) = Ok(cstate', acts) -> 
+    forall cstate cstate' chain ctx msg_payload acts,
+    (* a successful call *)
+    receive contract chain ctx cstate (Some (unpool (msg_payload))) = Ok(cstate', acts) -> 
+    (* an exchange rate exists *)
     exists r_x,
     FMap.find msg_payload.(token_unpooled) (stor_rates cstate) = Some r_x.
 
+Definition unpool_entrypoint_check_3 (contract : Contract Setup Msg State Error) : Prop :=
+    forall cstate cstate' chain ctx msg_payload acts,
+    (* a successful call *)
+    receive contract chain ctx cstate (Some (unpool (msg_payload))) = Ok(cstate', acts) -> 
+    (* an exchange rate exists *)
+    qty_unpooled msg_payload <=
+    get_rate (token_unpooled msg_payload) (stor_rates cstate) * get_bal (token_unpooled msg_payload) (stor_tokens_held cstate) / 1_000_000.
 
-(* When the UNPOOL entrypoint is successfully called, it emits a BURN call to the 
+(* When the WITHDRAW entrypoint is successfully called, it emits a BURN call to the 
     pool_token, with q in the payload *)
-Definition unpool_emits_burn (contract : Contract Setup Msg State Error) : Prop :=
-    forall bstate caddr cstate chain ctx msg msg_payload cstate' acts,
-    (* reachable bstate *)
-    reachable bstate -> 
-    (* the contract address is caddr with state cstate *)
-    env_contracts bstate caddr = Some (contract : WeakContract) -> 
-    contract_state bstate caddr = Some cstate -> 
-    (* the call to UNPOOL was successful *)
-    msg = unpool msg_payload -> 
-    receive contract chain ctx cstate (Some msg) = Ok(cstate', acts) -> 
-    (* in the acts list there is a BURN call with q in the payload *)
-    exists burn_data burn_payload,
-    (* there is a mint call in acts *)
-    In 
-    (act_call
-        (stor_pool_token cstate).(FA2Spec.token_address) (* calls the pool token address *)
-        0 (* with amount 0 *)
-        (serialize (FA2Spec.Retire burn_payload)))
-    acts /\ 
+Definition unpool_emits_txns (contract : Contract Setup Msg State Error) : Prop :=
+    forall cstate chain ctx msg_payload cstate' acts,
+    (* the call to WITHDRAW was successful *)
+    receive contract chain ctx cstate (Some (unpool msg_payload)) = Ok(cstate', acts) -> 
+    (* in the acts list there are burn and transfer transactions *)
+    exists burn_data burn_payload transfer_to transfer_data transfer_payload,
+    (* there is a burn call in acts *)
+    let burn_call := (act_call
+        (* calls the pool token address *)
+        (stor_pool_token cstate).(FA2Spec.token_address)
+        (* with amount 0 *)
+        0
+        (* with payload burn_payload *)
+        (serialize (FA2Spec.Retire burn_payload))) in 
     (* with has burn_data in the payload *)
     In burn_data burn_payload /\
     (* and burn_data has these properties: *)
     burn_data.(FA2Spec.retire_amount) = msg_payload.(qty_unpooled) /\
     (* the burned tokens go from the unpooler *)
-    burn_data.(FA2Spec.retiring_party) = ctx.(ctx_from).
-
-
-(* When the UNPOOL entrypoint is successfully called, it emits a TRANSFER call to the 
-    token in storage, with q * 1_000_000 / r_x tokens in the payload of the call *)
-Definition unpool_emits_transfer (contract : Contract Setup Msg State Error) : Prop :=
-    forall bstate caddr cstate chain ctx msg msg_payload cstate' acts,
-    (* reachable bstate *)
-    reachable bstate -> 
-    (* the contract address is caddr with state cstate *)
-    env_contracts bstate caddr = Some (contract : WeakContract) -> 
-    contract_state bstate caddr = Some cstate -> 
-    (* the call to UNPOOL was successful *)
-    msg = unpool (msg_payload) -> 
-    receive contract chain ctx cstate (Some msg) = Ok(cstate', acts) -> 
-    (* in the acts list there is a transfer call with q tokens as the payload *)
-    exists transfer_to transfer_data transfer_payload,
+    burn_data.(FA2Spec.retiring_party) = ctx.(ctx_from) /\
     (* there is a transfer call *)
-    In 
-    (act_call 
-        (msg_payload.(token_unpooled).(FA2Spec.token_address)) (* call to the token address *)
-        0 (* with amount = 0 *)
-        (serialize (FA2Spec.Transfer transfer_payload)))
-    acts /\ 
+    let transfer_call := (act_call 
+        (* call to the token address *)
+        (msg_payload.(token_unpooled).(FA2Spec.token_address))
+        (* with amount = 0 *)
+        0 
+        (* with payload transfer_payload *)
+        (serialize (FA2Spec.Transfer transfer_payload))) in 
     (* with a transfer in it *)
     In transfer_data transfer_payload /\ 
     (* which itself has transfer data *)
     In transfer_to transfer_data.(FA2Spec.txs) /\
     (* whose quantity is the quantity pooled *)
     let r_x := get_rate msg_payload.(token_unpooled) (stor_rates cstate) in 
-    transfer_to.(FA2Spec.amount) = msg_payload.(qty_unpooled) * 1_000_000 / r_x.
+    transfer_to.(FA2Spec.amount) = msg_payload.(qty_unpooled) * 1_000_000 / r_x /\
+    (* and these are the only emitted transactions *)
+    (acts = [ burn_call ; transfer_call ] \/
+     acts = [ transfer_call ; burn_call ]).
 
 
 (* When the UNPOOL entrypoint is successfully called, tokens_held goes down appropriately *)
 Definition unpool_decreases_tokens_held (contract : Contract Setup Msg State Error) : Prop := 
     forall cstate chain ctx msg_payload cstate' acts,
-    (* the call to POOL was successful *)
+    (* the call to DEPOSIT was successful *)
     receive contract chain ctx cstate (Some (unpool msg_payload)) = Ok(cstate', acts) -> 
     (* in cstate', tokens_held has increased at token *)
     let token := msg_payload.(token_unpooled) in
-    let qty := msg_payload.(qty_unpooled) in
+    let r_x := get_rate token (stor_rates cstate) in 
+    let qty := msg_payload.(qty_unpooled) * 1_000_000 / r_x in
     let old_bal := get_bal token (stor_tokens_held cstate) in 
     let new_bal := get_bal token (stor_tokens_held cstate') in 
-    new_bal = old_bal - qty.
+    new_bal = old_bal - qty /\ 
+    forall t,
+    t <> token -> 
+    get_bal t (stor_tokens_held cstate) = 
+    get_bal t (stor_tokens_held cstate').
 
 (* When the UNPOOL entrypoint is successfully called, tokens_held goes down appropriately *)
 Definition unpool_rates_unchanged (contract : Contract Setup Msg State Error) : Prop := 
     forall cstate cstate' chain ctx msg_payload acts,
-    (* the call to POOL was successful *)
+    (* the call to DEPOSIT was successful *)
     receive contract chain ctx cstate (Some (unpool msg_payload)) = Ok(cstate', acts) -> 
     (* rates all stay the same *)
     forall t,
@@ -437,38 +381,32 @@ Definition unpool_rates_unchanged (contract : Contract Setup Msg State Error) : 
 
 Definition unpool_outstanding (contract : Contract Setup Msg State Error) : Prop := 
     forall cstate cstate' chain ctx msg_payload acts,
-    (* the call to POOL was successful *)
+    (* the call to DEPOSIT was successful *)
     receive contract chain ctx cstate (Some (unpool msg_payload)) = Ok(cstate', acts) -> 
     (* rates all stay the same *)
     let rate_in := get_rate msg_payload.(token_unpooled) (stor_rates cstate) in 
     let qty := msg_payload.(qty_unpooled) in 
     stor_outstanding_tokens cstate' = 
-    stor_outstanding_tokens cstate - 1000000 / rate_in * qty.
+    stor_outstanding_tokens cstate - qty.
 
-(* If the TRADE entrypoint is called, token_in_trade and token_out_trade must both be 
-    part of the semi-fungible family for the trade to succeed. *)
+(* A call to the TRADE entrypoint fails if either the token to be traded in or the token 
+    to be traded out is not in the rates map held in the storage (=> is not in T) *)
 Definition trade_entrypoint_check (contract : Contract Setup Msg State Error) : Prop :=
-    forall bstate caddr cstate chain ctx msg msg_payload,
-    (* reachable bstate *)
-    reachable bstate -> 
-    (* the contract address is caddr with state cstate *)
-    env_contracts bstate caddr = Some (contract : WeakContract) -> 
-    contract_state bstate caddr = Some cstate -> 
-    (* forall calls to the Pool entrypoint *)
-    msg = trade (msg_payload) -> 
-    (* the receive function returns an error if the token to be pooled is not in the 
-       rates map held in the storage (=> is not in the semi-fungible family) *)
+    forall cstate chain ctx msg_payload,
+    (* If there is no entry in the rates map for either token in the trade, *)
     ((FMap.find msg_payload.(token_in_trade) (stor_rates cstate) = None) \/
-    (FMap.find msg_payload.(token_out_trade) (stor_rates cstate) = None)) ->
-    receive contract chain ctx cstate (Some msg) = 
+     (FMap.find msg_payload.(token_out_trade) (stor_rates cstate) = None)) ->
+    (* the transaction fails. *)
+    receive contract chain ctx cstate (Some (trade (msg_payload))) = 
       Err(error_to_Error error_TOKEN_NOT_FOUND).
 
-
+(* A successful call to TRADE means that token_in_trade and token_out_trade have exchange 
+    rates (=> are in T) *)
 Definition trade_entrypoint_check_2 (contract : Contract Setup Msg State Error) : Prop :=
     forall cstate chain ctx msg_payload cstate' acts,
-    (* the receive function returns an error if the token to be pooled is not in the 
-       rates map held in the storage (=> is not in the semi-fungible family) *)
+    (* a successful call *)
     receive contract chain ctx cstate (Some (trade (msg_payload))) = Ok(cstate', acts) -> 
+    (* exchange rates exist *)
     exists x r_x r_y,
     ((FMap.find msg_payload.(token_in_trade) (stor_tokens_held cstate) = Some x) /\
     (FMap.find msg_payload.(token_in_trade) (stor_rates cstate) = Some r_x) /\
@@ -480,19 +418,13 @@ Definition trade_entrypoint_check_2 (contract : Contract Setup Msg State Error) 
     given by calculate_trade. The updated rate is also priced using the formula from
     calculate_trade. *)
 Definition trade_pricing_formula (contract : Contract Setup Msg State Error) : Prop := 
-    forall bstate caddr cstate chain ctx msg msg_payload t_x t_y q cstate' acts,
-    (* reachable bstate *)
-    reachable bstate -> 
-    (* the contract address is caddr with state cstate *)
-    env_contracts bstate caddr = Some (contract : WeakContract) -> 
-    contract_state bstate caddr = Some cstate -> 
+    forall cstate chain ctx msg_payload t_x t_y q cstate' acts,
     (* the TRADE entrypoint was called succesfully *)
-    msg = trade msg_payload -> 
     t_x = msg_payload.(token_in_trade) -> 
     t_y = msg_payload.(token_out_trade) -> 
     t_x <> t_y -> 
     q = msg_payload.(qty_trade) ->
-    receive contract chain ctx cstate (Some msg) = 
+    receive contract chain ctx cstate (Some (trade msg_payload)) = 
       Ok(cstate', acts) -> 
     (* calculate the diffs delta_x and delta_y *)
     let delta_x := 
@@ -506,6 +438,30 @@ Definition trade_pricing_formula (contract : Contract Setup Msg State Error) : P
     (* the diff delta_x and delta_y are correct *)
     delta_x = q /\
     delta_y = calc_delta_y rate_in rate_out q k x.
+
+
+Definition trade_update_rates (contract : Contract Setup Msg State Error) : Prop := 
+    forall cstate chain ctx msg_payload cstate' acts,
+    (* the TRADE entrypoint was called succesfully *)
+    receive contract chain ctx cstate (Some (trade msg_payload)) = 
+      Ok(cstate', acts) -> 
+    let t_x := msg_payload.(token_in_trade) in
+    let t_y := msg_payload.(token_out_trade) in
+    t_x <> t_y /\
+    (* calculate the diffs delta_x and delta_y *)
+    let rate_in := (get_rate t_x (stor_rates cstate)) in 
+    let rate_out := (get_rate t_y (stor_rates cstate)) in 
+    let q := msg_payload.(qty_trade) in
+    let k := (stor_outstanding_tokens cstate) in 
+    let x := get_bal t_x (stor_tokens_held cstate) in 
+    (* the new rate of t_x is correct *)
+    let r_x' := calc_rate_in rate_in rate_out q k x in 
+    (stor_rates cstate') = 
+    (FMap.add (token_in_trade msg_payload)
+        (calc_rate_in (get_rate (token_in_trade msg_payload) (stor_rates cstate))
+        (get_rate (token_out_trade msg_payload) (stor_rates cstate)) (qty_trade msg_payload)
+        (stor_outstanding_tokens cstate) (get_bal (token_in_trade msg_payload) (stor_tokens_held cstate)))
+        (stor_rates cstate)).
 
 
 Definition trade_update_rates_formula (contract : Contract Setup Msg State Error) : Prop := 
@@ -530,60 +486,41 @@ Definition trade_update_rates_formula (contract : Contract Setup Msg State Error
         FMap.find t (stor_rates cstate)).
 
 
-(* When TRADE is successfully called, it emits a TRANSFER action of t_x in quantity q *)
-Definition trade_emits_transfer_tx (contract : Contract Setup Msg State Error) : Prop :=
-    forall bstate caddr cstate cstate' chain ctx msg msg_payload acts,
-    (* reachable bstate *)
-    reachable bstate -> 
-    (* the contract address is caddr with state cstate *)
-    env_contracts bstate caddr = Some (contract : WeakContract) -> 
-    contract_state bstate caddr = Some cstate -> 
+(* When TRADE is successfully called, it emits two TRANSFER actions *)
+Definition trade_emits_transfers (contract : Contract Setup Msg State Error) : Prop :=
+    forall cstate cstate' chain ctx msg_payload acts,
     (* the call to TRADE was successful *)
-    msg = trade (msg_payload) -> 
-    receive contract chain ctx cstate (Some msg) = Ok(cstate', acts) -> 
-    (* in the acts list there is a transfer call with q tokens as the payload *)
-    exists transfer_to transfer_data transfer_payload,
-    (* there is a transfer call *)
-    In 
-    (act_call 
-        (msg_payload.(token_in_trade).(FA2Spec.token_address)) (* call to the correct token address *)
-        0 (* with amount = 0 *)
-        (serialize (FA2Spec.Transfer transfer_payload)))
-    acts /\ 
+    receive contract chain ctx cstate (Some (trade (msg_payload))) = Ok(cstate', acts) -> 
+    (* the acts list consists of two transfer actions, specified as follows: *)
+    exists transfer_to_x transfer_data_x transfer_payload_x
+           transfer_to_y transfer_data_y transfer_payload_y,
+    (* there is a transfer call for t_x *)
+    let transfer_tx := (act_call 
+        (* call to the correct token address *)
+        (msg_payload.(token_in_trade).(FA2Spec.token_address))
+        (* with amount = 0 *)
+        0
+        (* and payload transfer_payload_x *)
+        (serialize (FA2Spec.Transfer transfer_payload_x))) in 
     (* with a transfer in it *)
-    In transfer_data transfer_payload /\ 
+    In transfer_data_x transfer_payload_x /\ 
     (* which itself has transfer data *)
-    In transfer_to transfer_data.(FA2Spec.txs) /\
+    In transfer_to_x transfer_data_x.(FA2Spec.txs) /\
     (* whose quantity is the quantity traded, transferred to the contract *)
-    transfer_to.(FA2Spec.amount) = msg_payload.(qty_trade) /\
-    transfer_to.(FA2Spec.to_) = ctx.(ctx_contract_address).
-
-
-(* transfers with delta_y given by calculate_trade function *)
-Definition trade_emits_transfer_ty (contract : Contract Setup Msg State Error) : Prop :=
-    forall bstate caddr cstate chain ctx msg msg_payload cstate' acts,
-    (* reachable bstate *)
-    reachable bstate -> 
-    (* the contract address is caddr with state cstate *)
-    env_contracts bstate caddr = Some (contract : WeakContract) -> 
-    contract_state bstate caddr = Some cstate -> 
-    (* the call to TRADE was successful *)
-    msg = trade (msg_payload) -> 
-    receive contract chain ctx cstate (Some msg) = 
-      Ok(cstate', acts) -> 
-    (* in the acts list there is a transfer call with q tokens as the payload *)
-    exists transfer_to transfer_data transfer_payload,
-    (* there is a transfer call *)
-    In 
-    (act_call 
-        (msg_payload.(token_out_trade).(FA2Spec.token_address)) (* call to the correct token address *)
-        0 (* with amount = 0 *)
-        (serialize (FA2Spec.Transfer transfer_payload)))
-    acts /\ 
+    transfer_to_x.(FA2Spec.amount) = msg_payload.(qty_trade) /\
+    transfer_to_x.(FA2Spec.to_) = ctx.(ctx_contract_address) /\ 
+    (* there is a transfer call for t_y *)
+    let transfer_ty := (act_call 
+        (* call to the correct token address *)
+        (msg_payload.(token_out_trade).(FA2Spec.token_address))
+        (* with amount = 0 *)
+        0 
+        (* and payload transfer_payload_y *)
+        (serialize (FA2Spec.Transfer transfer_payload_y))) in 
     (* with a transfer in it *)
-    In transfer_data transfer_payload /\ 
+    In transfer_data_y transfer_payload_y /\ 
     (* which itself has transfer data *)
-    In transfer_to transfer_data.(FA2Spec.txs) /\
+    In transfer_to_y transfer_data_y.(FA2Spec.txs) /\
     (* whose quantity is the quantity traded, transferred to the contract *)
     let t_x := msg_payload.(token_in_trade) in 
     let t_y := msg_payload.(token_out_trade) in 
@@ -592,8 +529,12 @@ Definition trade_emits_transfer_ty (contract : Contract Setup Msg State Error) :
     let k := (stor_outstanding_tokens cstate) in 
     let x := get_bal t_x (stor_tokens_held cstate) in 
     let q := msg_payload.(qty_trade) in 
-    transfer_to.(FA2Spec.amount) = calc_delta_y rate_in rate_out q k x  /\
-    transfer_to.(FA2Spec.to_) = ctx.(ctx_from).
+    transfer_to_y.(FA2Spec.amount) = calc_delta_y rate_in rate_out q k x  /\
+    transfer_to_y.(FA2Spec.to_) = ctx.(ctx_from) /\ 
+    (* acts is only these two transfers *)
+    (acts = [ transfer_tx ; transfer_ty ] \/
+     acts = [ transfer_ty ; transfer_tx ]).
+
 
 Definition trade_tokens_held_update (contract : Contract Setup Msg State Error) : Prop :=
     forall cstate chain ctx msg_payload cstate' acts,
@@ -610,6 +551,7 @@ Definition trade_tokens_held_update (contract : Contract Setup Msg State Error) 
     let delta_y := calc_delta_y rate_in rate_out delta_x k x in 
     let prev_bal_y := get_bal t_y (stor_tokens_held cstate) in 
     let prev_bal_x := get_bal t_x (stor_tokens_held cstate) in 
+    (* balances update appropriately *)
     get_bal t_y (stor_tokens_held cstate') = (prev_bal_y - delta_y) /\
     get_bal t_x (stor_tokens_held cstate') = (prev_bal_x + delta_x) /\
     forall t_z, 
@@ -623,31 +565,28 @@ Definition trade_outstanding_update (contract : Contract Setup Msg State Error) 
     (* the call to TRADE was successful *)
     receive contract chain ctx cstate (Some (trade (msg_payload))) = Ok(cstate', acts) -> 
     (* in the new state *)
-    let t_x := msg_payload.(token_in_trade) in 
-    let t_y := msg_payload.(token_out_trade) in 
+    (stor_outstanding_tokens cstate') = (stor_outstanding_tokens cstate).
+
+Definition trade_pricing (contract : Contract Setup Msg State Error) : Prop :=
+    forall cstate chain ctx msg_payload cstate' acts,
+    (* the call to TRADE was successful *)
+    receive contract chain ctx cstate (Some (trade (msg_payload))) = Ok(cstate', acts) -> 
+    (* balances for t_x change appropriately *)
+    FMap.find (token_in_trade msg_payload) (stor_tokens_held cstate') =
+    Some (get_bal (token_in_trade msg_payload) (stor_tokens_held cstate) + (qty_trade msg_payload)) /\ 
+    (* balances for t_y change appropriately *)
+    let t_x := token_in_trade msg_payload in 
+    let t_y := token_out_trade msg_payload in 
+    let delta_x := qty_trade msg_payload in 
     let rate_in := (get_rate t_x (stor_rates cstate)) in 
     let rate_out := (get_rate t_y (stor_rates cstate)) in 
     let k := (stor_outstanding_tokens cstate) in 
-    let x := get_bal t_x (stor_tokens_held cstate) in 
-    let delta_x := msg_payload.(qty_trade) in 
-    let delta_y := calc_delta_y rate_in rate_out delta_x k x in 
-    (stor_outstanding_tokens cstate') = 
-    (stor_outstanding_tokens cstate) + delta_x - delta_y.
-
-Definition trade_in_deposit (contract : Contract Setup Msg State Error) : Prop :=
-    forall bstate caddr cstate chain ctx msg msg_payload cstate' acts,
-    (* reachable bstate *)
-    reachable bstate -> 
-    (* the contract address is caddr with state cstate *)
-    env_contracts bstate caddr = Some (contract : WeakContract) -> 
-    contract_state bstate caddr = Some cstate -> 
-    (* the call to TRADE was successful *)
-    msg = trade (msg_payload) -> 
-    receive contract chain ctx cstate (Some msg) = Ok(cstate', acts) -> 
+    let x := get_bal t_x (stor_tokens_held cstate) in
     (* in the new state *)
-    (* TODO COVER THE CASE THAT t_in = t_out *)
-    FMap.find (token_in_trade msg_payload) (stor_tokens_held cstate') =
-    Some (get_bal (token_in_trade msg_payload) (stor_tokens_held cstate) + (qty_trade msg_payload)).
+    FMap.find (token_out_trade msg_payload) (stor_tokens_held cstate') =
+    Some (get_bal (token_out_trade msg_payload) (stor_tokens_held cstate) 
+        - (calc_delta_y rate_in rate_out delta_x k x)).
+
 
 (*
 Definition stor_outstanding_tokens (contract : Contract Setup Msg State Error) : Prop :=
@@ -671,61 +610,79 @@ Definition stor_outstanding_tokens (contract : Contract Setup Msg State Error) :
 *)
 
 (* Initialization specification *)
-Definition initialized_with_nonzero_rates (contract : Contract Setup Msg State Error) : Prop := 
+Definition initialized_with_positive_rates (contract : Contract Setup Msg State Error) := 
     forall chain ctx setup cstate,
-    (* we call init successfully *)
+    (* If the contract initializes successfully *)
     init contract chain ctx setup = Ok cstate -> 
     (* then all rates are nonzero *)
     forall t r,
     FMap.find t (stor_rates cstate) = Some r -> 
     r > 0.
 
-Definition initialized_with_zero_balance (contract : Contract Setup Msg State Error) : Prop := 
+Definition initialized_with_zero_balance (contract : Contract Setup Msg State Error) := 
     forall chain ctx setup cstate,
-    (* we call init successfully *)
+    (* If the contract initializes successfully *)
     init contract chain ctx setup = Ok cstate -> 
-    (* then all rates are nonzero *)
+    (* then all token balances initialize to zero *)
     forall t,
     get_bal t (stor_tokens_held cstate) = 0.
 
-Definition initialized_with_zero_outstanding (contract : Contract Setup Msg State Error) : Prop := 
+Definition initialized_with_zero_outstanding (contract : Contract Setup Msg State Error) := 
     forall chain ctx setup cstate,
-    (* we call init successfully *)
+    (* If the contract initializes successfully *)
     init contract chain ctx setup = Ok cstate -> 
-    (* then all rates are nonzero *)
+    (* then there are no outstanding tokens *)
     stor_outstanding_tokens cstate = 0.
+
+Definition initialized_with_init_rates (contract : Contract Setup Msg State Error) := 
+    forall chain ctx setup cstate,
+    (* If the contract initializes successfully *)
+    init contract chain ctx setup = Ok cstate -> 
+    (* then the init rates map is the same as given in the setup *)
+    (stor_rates cstate) = (init_rates setup).
+
+Definition initialized_with_pool_token (contract : Contract Setup Msg State Error) := 
+    forall chain ctx setup cstate,
+    (* If the contract initializes successfully *)
+    init contract chain ctx setup = Ok cstate -> 
+    (* then the pool token is the same as given in the setup *)
+    (stor_pool_token cstate) = (init_pool_token setup).
 
 (* we amalgamate each proposition in the specification into a single proposition *)
 Definition is_structured_pool
     (C : Contract Setup Msg State Error) : Prop := 
     none_fails C /\
+    (* pool entrypoint specification *)
     pool_entrypoint_check C /\
     pool_entrypoint_check_2 C /\
-    pool_emits_transfer C /\
-    pool_emits_mint C /\
-    pool_atomic C /\
+    pool_emits_txns C /\
     pool_increases_tokens_held C /\
     pool_rates_unchanged C /\
     pool_outstanding C /\
+    (* unpool entrypoint specification *)
     unpool_entrypoint_check C /\
     unpool_entrypoint_check_2 C /\
-    unpool_emits_burn C /\
-    unpool_emits_transfer C /\
+    unpool_entrypoint_check_3 C /\
+    unpool_emits_txns C /\
     unpool_decreases_tokens_held C /\
     unpool_rates_unchanged C /\
     unpool_outstanding C /\
+    (* trade entrypoint specification *)
     trade_entrypoint_check C /\
     trade_entrypoint_check_2 C /\
     trade_pricing_formula C /\
+    trade_update_rates C /\
     trade_update_rates_formula C /\
-    trade_emits_transfer_tx C /\
-    trade_emits_transfer_ty C /\
+    trade_emits_transfers C /\
     trade_tokens_held_update C /\
     trade_outstanding_update C /\
-    trade_in_deposit C /\
-    initialized_with_nonzero_rates C /\
+    trade_pricing C /\ 
+    (* initialization specification *)
+    initialized_with_positive_rates C /\
     initialized_with_zero_balance C /\
-    initialized_with_zero_outstanding C.
+    initialized_with_zero_outstanding C /\ 
+    initialized_with_init_rates C /\ 
+    initialized_with_pool_token C.
 
 (* A tactic to destruct is_sp if it's in the context of a proof *)
 Tactic Notation "is_sp_destruct" := 
@@ -733,32 +690,36 @@ Tactic Notation "is_sp_destruct" :=
     | is_sp : is_structured_pool _ |- _ => 
         unfold is_structured_pool in is_sp;
         destruct is_sp  as [none_fails_pf is_sp'];
+        (* isolate the pool entrypoint specification *)
         destruct is_sp'  as [pool_entrypoint_check_pf is_sp'];
         destruct is_sp' as [pool_entrypoint_check_2_pf is_sp'];
-        destruct is_sp' as [pool_emits_transfer_pf is_sp'];
-        destruct is_sp' as [pool_emits_mint_pf is_sp'];
-        destruct is_sp' as [pool_atomic_pf is_sp'];
+        destruct is_sp' as [pool_emits_txns_pf is_sp'];
         destruct is_sp' as [pool_increases_tokens_held_pf is_sp'];
         destruct is_sp' as [pool_rates_unchanged_pf is_sp'];
         destruct is_sp' as [pool_outstanding_pf is_sp'];
+        (* isolate the unpool entrypoint specification *)
         destruct is_sp' as [unpool_entrypoint_check_pf is_sp'];
         destruct is_sp' as [unpool_entrypoint_check_2_pf is_sp'];
-        destruct is_sp' as [unpool_emits_burn_pf is_sp'];
-        destruct is_sp' as [unpool_emits_transfer_pf is_sp'];
+        destruct is_sp' as [unpool_entrypoint_check_3_pf is_sp'];
+        destruct is_sp' as [unpool_emits_txns_pf is_sp'];
         destruct is_sp' as [unpool_decreases_tokens_held_pf is_sp'];
         destruct is_sp' as [unpool_rates_unchanged_pf is_sp'];
         destruct is_sp' as [unpool_outstanding_pf is_sp'];
+        (* isolate the trade entrypoint specification *)
         destruct is_sp' as [trade_entrypoint_check_pf is_sp'];
         destruct is_sp' as [trade_entrypoint_check_2_pf is_sp'];
         destruct is_sp' as [trade_pricing_formula_pf is_sp'];
+        destruct is_sp' as [trade_update_rates_pf is_sp'];
         destruct is_sp' as [trade_update_rates_formula_pf is_sp'];
-        destruct is_sp' as [trade_emits_transfer_tx_pf is_sp'];
-        destruct is_sp' as [trade_emits_transfer_ty_pf is_sp'];
+        destruct is_sp' as [trade_emits_transfers is_sp'];
         destruct is_sp' as [trade_tokens_held_update_pf is_sp']; 
         destruct is_sp' as [trade_outstanding_update_pf is_sp'];
-        destruct is_sp' as [trade_in_deposit_pf is_sp'];
-        destruct is_sp' as [initialized_with_nonzero_rates_pf is_sp']; 
-        destruct is_sp' as [initialized_with_zero_balance_pf initialized_with_zero_outstanding_pf]
+        destruct is_sp' as [trade_pricing is_sp'];
+        (* isolate the initialization specification *)
+        destruct is_sp' as [initialized_with_positive_rates_pf is_sp']; 
+        destruct is_sp' as [initialized_with_zero_balance_pf is_sp']; 
+        destruct is_sp' as [initialized_with_zero_outstanding_pf is_sp'];
+        destruct is_sp' as [initialized_with_init_rates_pf initialized_with_pool_token_pf]
 end.
 
 
@@ -770,44 +731,48 @@ end.
  * ============================================================================= *)
 
 Context {contract : Contract Setup Msg State Error}
-        { is_sp : is_structured_pool contract }
-        (* some common assumptions in the metaspecification *)
+        { is_sp : is_structured_pool contract }.
+        (* some common assumptions in the metaspecification 
         { bstate : ChainState } { caddr : Address } { cstate : State }
         (* reachable state *)
         { reachable_st : reachable bstate } { trace : ChainTrace empty_state bstate}
         (* with contract at caddr *)
         { contract_at_caddr : env_contracts bstate caddr = Some (contract : WeakContract) }
         (* with contract state cstate *)
-        { state_is_cstate : contract_state bstate caddr = Some cstate }.
+        { state_is_cstate : contract_state bstate caddr = Some cstate }.*)
 
 (* Some assumptions (should probably prove some of these) *)
-(* update_rate function returns positive number  *)
-Axiom update_rate_returns_positive : forall r_x r_y delta_x k x, 
+(* update_rate function returns positive number if the num, denom are positive *)
+Lemma update_rate_returns_positive : forall r_x r_y delta_x k x, 
     let r_x' := calc_rate_in r_x r_y delta_x k x in
     let delta_y := calc_delta_y r_x r_y delta_x k x in  
     (r_x * x / 1_000_000 + r_y * delta_y / 1_000_000) > 0 -> 
     (x + delta_x) > 0 -> 
     r_x' > 0.
+Admitted.
 
+(* TODO Lemma-tize *)
 Axiom update_rate_stays_positive : forall r_x r_y delta_x k x, 
     let r_x' := calc_rate_in r_x r_y delta_x k x in
     r_x > 0 ->
     r_x' > 0.
 
 (* calculate_trade function returns a positive number if k, r_x, r_y, delta_x > 0 *)
-Axiom calc_trade_returns_positive : forall r_x r_y delta_x k x, 
+Lemma calc_trade_returns_positive : forall r_x r_y delta_x k x, 
     k > 0 -> 
     r_x > 0 -> 
     r_y > 0 -> 
     delta_x > 0 -> 
     calc_delta_y r_x r_y delta_x k x > 0.
+Admitted.
 
 (* r_x' < r_x *)
-Axiom rate_decrease : forall r_x r_y delta_x k x, 
+Lemma rate_decrease : forall r_x r_y delta_x k x, 
     let r_x' := calc_rate_in r_x r_y delta_x k x in 
     r_x' < r_x.
+Admitted.
 
-(* delta_y < ( r_y / r_x ) * delta_x *)
+(* Assumed: delta_y < ( r_y / r_x ) * delta_x *)
 Axiom trade_upper_bound : forall r_x r_y delta_x k x, 
     let delta_y := calc_delta_y r_x r_y delta_x k x in 
     delta_y < ( r_y / r_x ) * delta_x.
@@ -826,6 +791,7 @@ Lemma arbitrage_lemma_lt :
     calc_rate_in rate_x rate_y delta_x k x <= ext.
 Admitted.
 
+(* TODO THIS IS FALSE, the one you have to choose is the actual balance that you have, then it depletes. *)
 Lemma arbitrage_lemma_gt : 
     forall rate_x rate_y ext k x,
     ext > rate_x -> 
@@ -891,7 +857,7 @@ Proof.
     exact x_leq.
 Qed.
 
-Theorem demand_sensitivity :
+Theorem demand_sensitivity cstate :
     (* For all tokens t_x t_y, rates r_x r_y, and quantities x and y, where *)
     forall t_x r_x x t_y r_y y,
     (* t_x is a token with nonzero pooled liquidity and with rate r_x > 0, and *)
@@ -1012,20 +978,25 @@ Qed.
     of CPMMs.
 *)
 
-Theorem nonpathological_prices : 
+Theorem nonpathological_prices bstate caddr :
+    (* reachable state with contract at caddr *)
+    reachable bstate -> 
+    env_contracts bstate caddr = Some (contract : WeakContract) ->
+    (* the statement *)
     exists (cstate : State),
     contract_state bstate caddr = Some cstate /\
     (* For a token t_x in T and rate r_x, *)
     forall t_x r_x,
-    (* such that in the contract state cstate the rate of t_x is r_x and r_x > 0, *)
+    (* if r_x is the exchange rate of t_x, then r_x > 0 *)
     FMap.find t_x (stor_rates cstate) = Some r_x -> r_x > 0.
 Proof.
+    intros reachable_st contract_at_caddr.
     contract_induction; intros.
     (* Please reestablish the invariant after addition of a block *)
     -   exact (IH t_x r_x H6).
     (* Please establish the invariant after deployment of the contract *)
     -   is_sp_destruct. clear is_sp.
-        pose proof (initialized_with_nonzero_rates_pf chain ctx setup result init_some) as init_rates.
+        pose proof (initialized_with_positive_rates_pf chain ctx setup result init_some) as init_rates.
         exact (init_rates t_x r_x H6).
     (* Please reestablish the invariant after an outgoing action *)
     -   exact (IH t_x r_x H6).
@@ -1249,7 +1220,7 @@ Fixpoint are_successive_trades (trade_sequence : list trade_sequence_type) : Pro
     end.
 
 (* a function to calculate the the trade output of the final trade, delta_x' *)
-Definition calc_final_delta (t : trade_sequence_type) := 
+Definition trade_to_delta_y (t : trade_sequence_type) := 
     let cstate := seq_cstate t in 
     let token_in := token_in_trade (seq_trade_data t) in 
     let token_out := token_out_trade (seq_trade_data t) in 
@@ -1261,56 +1232,30 @@ Definition calc_final_delta (t : trade_sequence_type) :=
     (* the calculation *)
     calc_delta_y rate_in rate_out delta_x k x.
 
-Definition swap_rate_lemma : 
-    forall t_x r_x x t_y r_y y, 
-    (* t_x is a token with nonzero pooled liquidity and with rate r_x > 0, and *)
-    FMap.find t_x (stor_tokens_held cstate) = Some x /\ x > 0 /\
-    FMap.find t_x (stor_rates cstate) = Some r_x /\ r_x > 0 ->
-    (* t_y is a token with nonzero pooled liquidity and with rate r_y > 0 *)
-    FMap.find t_y (stor_tokens_held cstate) = Some y /\ y > 0 /\
-    FMap.find t_y (stor_rates cstate) = Some r_y /\ r_y > 0 ->
-    (* In a trade t_x to t_y ... *)
-    forall chain ctx msg msg_payload acts cstate',
-        (* i.e.: a successful call to the contract *)
-        receive contract chain ctx cstate (Some msg) = Ok(cstate', acts) ->
-        (* which is a trade *)
-        msg = trade msg_payload ->
-        (* from t_x to t_y *)
-        msg_payload.(token_in_trade) = t_x ->
-        msg_payload.(token_out_trade) = t_y ->
-        (* with t_x <> t_y *)
-        t_x <> t_y -> 
-    (* ... as r_x is updated to r_x': ... *)
-    let delta_x := msg_payload.(qty_trade) in 
-    let delta_y := calc_delta_y r_x r_y delta_x (stor_outstanding_tokens cstate) x in 
-    let r_x' := get_rate t_x (stor_rates cstate') in 
-    r_y * delta_y <= r_x' * delta_x.
-Proof.
-    intros * lqty_x lqty_y * trade_success msg_is_trade from_tx to_ty tx_neq_ty *.
-    is_sp_destruct. clear is_sp.
-    rewrite msg_is_trade in trade_success.
-    pose proof (trade_update_rates_formula_pf cstate chain ctx msg_payload cstate' acts
-        trade_success)
-    as rx_update.
-    simpl in rx_update.
-    destruct rx_update as [_ rates_update].
-    simpl in rates_update.
-    destruct rates_update as [tx_update tz_update].
-    assert (r_x' = calc_rate_in r_x r_y (qty_trade msg_payload) (stor_outstanding_tokens cstate) x) as r_x'_calc.
-    { admit. }
-    rewrite r_x'_calc.
-    unfold calc_rate_in.
-    assert (forall x1 x2 y z : N, z <= x1 / y * x2 <-> z * y <= x1 * x2) as div_alg. 
-    { admit. }
-    rewrite (div_alg 
-        (r_x * x / 1000000 + r_y * calc_delta_y r_x r_y (qty_trade msg_payload) (stor_outstanding_tokens cstate) x / 1000000)
-        delta_x
-        (x + qty_trade msg_payload)
-        (r_y * delta_y)).
-Admitted.
+Fixpoint leq_list (l : list N) : Prop := 
+    match l with 
+    | [] => True 
+    | h :: tl => 
+        match tl with 
+        | [] => True 
+        | h' :: tl' => (h <= h') /\ leq_list tl 
+        end 
+    end.
+
+Definition trade_to_ry_delta_y (t : trade_sequence_type) := 
+    let delta_y := trade_to_delta_y t in 
+    let rate_y := get_rate (token_out_trade (seq_trade_data t)) (stor_rates (seq_cstate t)) in 
+    rate_y * delta_y.
+
+Lemma swap_rate_lemma (trade_sequence : list trade_sequence_type) : 
+    (* if this is a list of successive trades *)
+    are_successive_trades trade_sequence -> 
+    (* then  *)
+    leq_list (map trade_to_ry_delta_y trade_sequence).
+Admitted. 
 
 
-Theorem swap_rate_consistency : 
+Theorem swap_rate_consistency bstate cstate : 
     (* Let t_x be a token with nonzero pooled liquidity and rate r_x > 0 *)
     forall t_x r_x x,
     FMap.find t_x (stor_rates cstate) = Some r_x /\ r_x > 0 /\ 
@@ -1331,7 +1276,7 @@ Theorem swap_rate_consistency :
     (* the last trade is to t_x *)
     token_out_trade (seq_trade_data t_last) = t_x -> 
     (* delta_x', the output of the last trade, is never larger than delta_x. *)
-    let delta_x' := calc_final_delta t_last in 
+    let delta_x' := trade_to_delta_y t_last in 
     delta_x' <= delta_x.
 Proof.
     (* from paper: 
@@ -1356,12 +1301,13 @@ Proof.
     (* TODO a function that gives this for any n. Define the function recursively. *)
 Admitted.
 
+
 (* Zero-Impact Liquidity Change :
     The quoted price of trades is unaffected by calling DEPOSIT and WITHDRAW 
 *)
-Theorem zero_impact_liquidity_change_deposit :
+Theorem zero_impact_liquidity_change :
     (* Consider the quoted price of a trade t_x to t_y at cstate, *)
-    forall t_x t_y r_x r_y,
+    forall cstate t_x t_y r_x r_y,
     FMap.find t_x (stor_rates cstate) = Some r_x ->
     FMap.find t_y (stor_rates cstate) = Some r_y ->
     let quoted_price := r_x / r_y in 
@@ -1448,7 +1394,7 @@ Qed.
     sensitivity or the pool depletes in that particular token.
 *)
 Theorem arbitrage_sensitivity :
-    forall t_x r_x x,
+    forall cstate t_x r_x x,
     (* t_x is a token with nonzero pooled liquidity *)
     FMap.find t_x (stor_rates cstate) = Some r_x /\ r_x > 0 /\ 
     FMap.find t_x (stor_tokens_held cstate) = Some x /\ x > 0 ->
@@ -1561,40 +1507,188 @@ Qed.
     pooled tokens, always equals the total number of outstanding pool tokens. That is, 
     pool tokens are never under- or over-collateralized. 
 *)
-Definition fold_fn (rates : FMap token exchange_rate) (tokens_held : FMap token N)
-    (n : N) (k : token) : N := 
-    let rate := 
-        match FMap.find k rates with 
-        | Some r => r 
-        | None => 0
-        end in 
-    let qty_held := 
-        match FMap.find k tokens_held with 
-        | Some r => r 
-        | None => 0 
-        end in 
-    rate * qty_held / 1_000_000.
 
-Definition sum_over_tokens 
-    (rates : FMap token exchange_rate) (tokens_held : FMap token N) : N := 
-    (* get the list of keys *)
-    let token_family := (FMap.keys rates) in 
-    (* fold over the list *)
-    List.fold_left
-        (fold_fn rates tokens_held)
-        token_family 
-        0.
+(* map over the keys *)
+Definition tokens_to_values (rates : FMap token exchange_rate) (tokens_held : FMap token N) : list N := 
+    List.map
+        (fun k => 
+            let rate := get_rate k rates in 
+            let qty_held := get_bal k tokens_held in 
+            rate * qty_held / 1_000_000)
+        (FMap.keys rates).
 
-Theorem pooled_consistency : 
+(* some lemmas *)
+Lemma token_keys_invariant_pool : forall p new_state new_acts prev_state ctx chain,
+    receive contract chain ctx prev_state (Some (pool p)) =
+        Ok (new_state, new_acts) -> 
+    (FMap.keys (stor_rates new_state)) = 
+    (FMap.keys (stor_rates prev_state)).
+Proof.
+    intros * receive_some.
+    is_sp_destruct.
+    (* pool p *)
+    pose proof (pool_rates_unchanged_pf prev_state new_state chain ctx p new_acts receive_some) as rates_unchanged.
+        assert ((stor_rates prev_state) = (stor_rates new_state)) as rates_eq.
+        {   apply FMap.ext_eq.
+            auto. }
+        rewrite <- rates_eq.
+    reflexivity.
+Qed.
+
+Lemma token_keys_invariant_unpool : forall u new_state new_acts prev_state ctx chain,
+    receive contract chain ctx prev_state (Some (unpool u)) =
+        Ok (new_state, new_acts) -> 
+    (FMap.keys (stor_rates new_state)) = 
+    (FMap.keys (stor_rates prev_state)).
+Proof.
+    intros * receive_some.
+    is_sp_destruct.
+    (* unpool u *)
+    pose proof (unpool_rates_unchanged_pf prev_state new_state chain ctx u new_acts receive_some) as unrates_unchanged.
+        assert ((stor_rates prev_state) = (stor_rates new_state)) as rates_eq.
+        {   apply FMap.ext_eq.
+            auto. }
+        rewrite <- rates_eq.
+    reflexivity.
+Qed.
+
+Lemma token_keys_invariant_trade : forall t new_state new_acts prev_state ctx chain,
+    receive contract chain ctx prev_state (Some (trade t)) =
+        Ok (new_state, new_acts) -> 
+    Permutation 
+    (FMap.keys (stor_rates new_state))
+    (FMap.keys (stor_rates prev_state)).
+Proof.
+    intros * receive_some.
+    is_sp_destruct.
+    (* trade t *)
+    pose proof (trade_update_rates_formula_pf prev_state chain ctx t new_state new_acts receive_some) 
+    as update_rates_formula.
+    destruct update_rates_formula as [tokens_neq update_rates_formula].
+    destruct update_rates_formula as [old_rate_in other_rates_unchanged].
+    (* ... *)
+    pose proof (trade_entrypoint_check_2_pf prev_state
+    chain ctx t new_state new_acts receive_some) 
+    as trade_check.
+    do 3 destruct trade_check as [* trade_check].
+    destruct trade_check as [_ trade_check]. 
+    destruct trade_check as [trade_check _].
+    clear x1 x.
+    pose proof (FMap.keys_already 
+        (token_in_trade t) x0 
+        (calc_rate_in
+            (get_rate (token_in_trade t)
+                (stor_rates prev_state))
+            (get_rate (token_out_trade t)
+                (stor_rates prev_state)) 
+            (qty_trade t)
+            (stor_outstanding_tokens prev_state)
+            (get_bal (token_in_trade t)
+                (stor_tokens_held prev_state)))
+        (stor_rates prev_state) trade_check)
+    as keys_permuted.
+    pose proof (trade_update_rates_pf prev_state chain ctx t new_state new_acts receive_some)
+    as update_rates.
+    destruct update_rates as [_ update_rates].
+    simpl in update_rates.
+    (* rewrite <- update_rates in H6 *)
+    replace (FMap.add (token_in_trade t)
+        (calc_rate_in (get_rate (token_in_trade t) (stor_rates prev_state))
+        (get_rate (token_out_trade t) (stor_rates prev_state)) (qty_trade t)
+        (stor_outstanding_tokens prev_state) (get_bal (token_in_trade t) (stor_tokens_held prev_state)))
+        (stor_rates prev_state))
+    with (stor_rates new_state)
+    in keys_permuted.
+    exact keys_permuted.
+Qed.
+
+Definition suml l := fold_right N.add 0 l.
+
+(* and suml commutes with the permutation *)
+Lemma map_extract { A B : Type } : forall (a : A) (l : list A) (f : A -> B),
+    map f (a :: l) = 
+    (f a) :: map f l.
+Proof. auto. Qed.
+
+Lemma suml_extract : forall a l,
+    suml (a :: l) = 
+    a + (suml l).
+Proof. auto. Qed.
+
+Lemma in_map : forall { A B : Type } (f : A -> B) l a,
+    In a l -> In (f a) (map f l).
+Proof.
+    intros * H_in.
+    induction l as [|x l IH]; auto.
+    simpl. simpl in H_in. destruct H_in.
+    + left. subst. reflexivity.
+    + right. apply IH. assumption.
+Qed.
+
+Lemma nodup_permute : forall { A : Type } a (l : list A)
+    (eq_dec : forall a b, { a = b } + { a <> b }),
+    NoDup l -> 
+    In a l -> 
+    Permutation l (a :: remove eq_dec a l).
+Proof.
+    intros A a l eq_dec NoDup_l In_a_l.
+    induction NoDup_l as [| b l H_not_in_b_l NoDup_l IH].
+    - simpl in In_a_l. contradiction.
+    - simpl in In_a_l. destruct In_a_l as [a_eq_b | a_in_l].
+        + subst b. simpl. destruct (eq_dec a a).
+            * (* apply Permutation_refl. *) admit.
+            * contradiction.
+        + simpl. destruct (eq_dec a b).
+            * subst b. contradiction.
+            * apply Permutation_trans with (b :: a :: remove eq_dec a l).
+                { (* apply perm_swap. *) admit. }
+                { (* apply perm_skip. apply IH. assumption. *) admit. }
+Admitted.
+
+Lemma mapped_eq : forall (A B : Type) (f f' : A -> B) (l : list A),
+    (forall a, In a l -> f a = f' a) -> 
+    map f l = map f' l.
+Proof.
+    intros * H_in.
+    induction l; auto.
+    repeat rewrite map_extract.
+    rewrite (H_in a (in_eq a l)).
+    assert (forall a : A, In a l -> f a = f' a) as H_in_ind.
+    {   intros * in_a0.
+        exact (H_in a0 (in_cons a a0 l in_a0)). }
+    rewrite (IHl H_in_ind).
+    reflexivity.
+Qed.
+
+Lemma suml_permute_commutes : forall l l',
+    Permutation l l' -> suml l = suml l'.
+Proof.
+    intros. induction H6; auto.
+    -   repeat rewrite (suml_extract x).
+        rewrite IHPermutation.
+        reflexivity.
+    -   rewrite (suml_extract y). rewrite (suml_extract x).
+        rewrite (suml_extract x). rewrite (suml_extract y).
+        repeat rewrite N.add_assoc.
+        rewrite (N.add_comm x y).
+        reflexivity.
+    -   rewrite IHPermutation1.  
+        rewrite IHPermutation2.
+        reflexivity.
+Qed.
+
+Theorem pooled_consistency bstate caddr :
+    reachable bstate -> 
+    env_contracts bstate caddr = Some (contract : WeakContract) -> 
     exists (cstate : State),
     contract_state bstate caddr = Some cstate /\
     (* The sum of all the constituent, pooled tokens, multiplied by their value in terms 
     of pooled tokens, always equals the total number of outstanding pool tokens. *)
-    sum_over_tokens (stor_rates cstate) (stor_tokens_held cstate) = 
+    suml (tokens_to_values (stor_rates cstate) (stor_tokens_held cstate)) = 
         (stor_outstanding_tokens cstate).
 Proof.
     contract_induction; intros; try exact IH.
-    is_sp_destruct. clear is_sp.
+    is_sp_destruct.
     (* Please establish the invariant after deployment of the contract *)
     -   (* we use the fact that balances initialize at zero *)
         pose proof (initialized_with_zero_balance_pf chain ctx setup result init_some)
@@ -1602,125 +1696,402 @@ Proof.
         pose proof (initialized_with_zero_outstanding_pf chain ctx setup result init_some)
         as zero_outstanding.
         rewrite zero_outstanding. clear zero_outstanding.
-        unfold sum_over_tokens.
-        unfold fold_fn.
-        assert (forall k, match FMap.find k (stor_tokens_held result) with
-        | Some r => r
-        | None => 0
-        end = 0)
-        as no_tokens_held.
-        {   intro. 
-            unfold get_bal in zero_bal.
-            pose proof (zero_bal k) as e.
-            destruct (FMap.find k (stor_tokens_held result)).
-            exact e. 
-            reflexivity. }
-        assert ((fun (_ : N) (k : token) =>
-        match FMap.find k (stor_rates result) with
-        | Some r => r
-        | None => 0
-        end * match FMap.find k (stor_tokens_held result) with
-              | Some r => r
-              | None => 0
-              end / 1000000) = (fun (_ : N) (k : token) => 0))
-        as fold_fn_0.
-        {   apply functional_extensionality. 
-            intro n.
-            apply functional_extensionality. 
-            intro t.
-            rewrite (no_tokens_held t).
-            rewrite (N.mul_0_r (match FMap.find t (stor_rates result) with
-            | Some r => r
-            | None => 0
-            end)).
-            assert (1000000 <> 0) as neq_n. { auto. }
-            exact (N.div_0_l 1000000 neq_n). }
-        rewrite fold_fn_0.
-        unfold fold_left.
+        unfold tokens_to_values.
         induction (FMap.keys (stor_rates result)); auto.
+        rewrite map_cons.
+        rewrite zero_bal.
+        rewrite N.mul_0_r. 
+        auto.
     (* Please reestablish the invariant after a nonrecursive call *)
     -   destruct msg.
-        (* msg = Some m *)
-        +   destruct m.
-            (* m = pool *)
-            *   is_sp_destruct. clear is_sp.
-                (* understand how tokens_held has changed *)
-                pose proof (pool_increases_tokens_held_pf prev_state chain ctx p new_state new_acts
-                    receive_some) as bal_update.
-                simpl in bal_update.
-                (* show all rates are the same *)
-                pose proof (pool_rates_unchanged_pf prev_state new_state chain ctx p new_acts
-                    receive_some) as rates_update.
-                (* show how the outstanding tokens update *)
-                pose proof (pool_outstanding_pf prev_state new_state chain ctx p new_acts 
-                    receive_some) as out_update.
-                simpl in out_update.
-                assert (sum_over_tokens (stor_rates new_state) (stor_tokens_held new_state) = 
-                    sum_over_tokens (stor_rates prev_state) (stor_tokens_held new_state))
-                as rates_unchanged.
-                { admit. }
-                rewrite rates_unchanged. clear rates_unchanged.
-                assert (sum_over_tokens (stor_rates prev_state) (stor_tokens_held new_state) = 
-                    sum_over_tokens (stor_rates prev_state) (stor_tokens_held prev_state) + 
-                    get_rate (token_pooled p) (stor_rates prev_state) / 1000000 * qty_pooled p)
-                as separate_sum.
-                { admit. }
-                rewrite separate_sum. clear separate_sum.
-                rewrite out_update.
-                rewrite IH.
-                reflexivity.
-            (* m = unpool *)
-            *   is_sp_destruct. clear is_sp.
-                (* understand how tokens_held has changed *)
-                pose proof (unpool_decreases_tokens_held_pf prev_state chain ctx u new_state new_acts
-                    receive_some) as bal_update.
-                simpl in bal_update.
-                (* show all rates are the same *)
-                pose proof (unpool_rates_unchanged_pf prev_state new_state chain ctx u new_acts
-                    receive_some) as rates_update.
-                (* show how the outstanding tokens update *)
-                pose proof (unpool_outstanding_pf prev_state new_state chain ctx u new_acts 
-                    receive_some) as out_update.
-                simpl in out_update.
-                assert (sum_over_tokens (stor_rates new_state) (stor_tokens_held new_state) = 
-                    sum_over_tokens (stor_rates prev_state) (stor_tokens_held new_state))
-                as rates_unchanged.
-                { admit. }
-                rewrite rates_unchanged. clear rates_unchanged.
-                assert (sum_over_tokens (stor_rates prev_state) (stor_tokens_held new_state) = 
-                    sum_over_tokens (stor_rates prev_state) (stor_tokens_held prev_state) - 
-                    1000000 / get_rate (token_unpooled u) (stor_rates prev_state) * qty_unpooled u)
-                as separate_sum.
-                { admit. }
-                rewrite separate_sum. clear separate_sum.
-                rewrite out_update.
-                rewrite IH.
-                reflexivity.
-            (* m = trade *)
-            *   is_sp_destruct. clear is_sp.
-                (* understand how tokens_held has changed *)
-                pose proof (trade_tokens_held_update_pf prev_state chain ctx t new_state new_acts 
-                    receive_some) as tokens_held_update.
-                destruct tokens_held_update as [tokens_held_update_ty tokens_held_update].
-                destruct tokens_held_update as [tokens_held_update_tx tokens_held_update_tz].
-                (* how calling trade updates rates *)
-                pose proof (trade_update_rates_formula_pf prev_state chain ctx t new_state new_acts
-                    receive_some) as rates_changed_and_unchanged.
-                destruct rates_changed_and_unchanged as [tx_neq_ty rates_changed_and_unchanged].
-                destruct rates_changed_and_unchanged as [rx_change rz_unchanged].
-                (* how outstanding_tokens has changed by calling trade *)
-                pose proof (trade_outstanding_update_pf prev_state chain ctx t new_state new_acts 
-                    receive_some) as out_update.
-                (* LHS equals sum over tokens except for tx and ty, plus r_x' * etc , minus r_y * delta_y *)
-                admit.
-        (* msg = None *)
-        +   is_sp_destruct. clear is_sp.
+        (* first, msg = None *)
+        2:{ is_sp_destruct.
             pose proof (none_fails_pf prev_state chain ctx) as failed.
             destruct failed as [err failed].
             rewrite receive_some in failed.
-            inversion failed.
+            inversion failed. }
+        (* msg = Some m *)
+        destruct m.
+        (* m = pool *)
+        +   is_sp_destruct.
+            (* understand how tokens_held has changed *)
+            pose proof (pool_increases_tokens_held_pf prev_state chain ctx p new_state new_acts
+                receive_some) as bal_update.
+            destruct bal_update as [bal_update bals_unchanged].
+            (* show all rates are the same *)
+            pose proof (pool_rates_unchanged_pf prev_state new_state chain ctx p new_acts
+                receive_some) as rates_update.
+            (* show how the outstanding tokens update *)
+            pose proof (pool_outstanding_pf prev_state new_state chain ctx p new_acts 
+                receive_some) as out_update.
+            simpl in out_update.
+            (* because the rates are unchanged, summing over them is unchanged *)
+            assert (tokens_to_values (stor_rates new_state)  (stor_tokens_held new_state) = 
+                    tokens_to_values (stor_rates prev_state) (stor_tokens_held new_state))
+            as rates_unchanged.
+            {   unfold tokens_to_values.
+                rewrite (token_keys_invariant_pool p new_state new_acts prev_state ctx chain receive_some).
+                apply map_ext.
+                intro t.
+                unfold get_rate. rewrite rates_update.
+                auto.  }
+            rewrite rates_unchanged. clear rates_unchanged.
+            (* now separate the sum *)
+            assert (suml (tokens_to_values (stor_rates prev_state) (stor_tokens_held new_state)) = 
+                    suml (tokens_to_values (stor_rates prev_state) (stor_tokens_held prev_state)) + 
+                        get_rate (token_pooled p) (stor_rates prev_state) / 1000000 * qty_pooled p)
+            as separate_sum.
+            {   unfold tokens_to_values.
+                (* some simplifying notation *)
+                set (keys_minus_p := (remove token_eq_dec (token_pooled p) (FMap.keys (stor_rates prev_state)))).
+                set (tokens_to_values_new := fun k : token => get_rate k (stor_rates prev_state) * get_bal k (stor_tokens_held new_state) / 1000000).
+                set (tokens_to_values_prev := fun (k : token) => get_rate k (stor_rates prev_state) * get_bal k (stor_tokens_held prev_state) / 1000000).
+                (* 1. show there's a Permutation with (token_pooled p) at the front *)
+                assert (Permutation
+                    (FMap.keys (stor_rates prev_state)) 
+                    ((token_pooled p) :: keys_minus_p))
+                as keys_permuted.
+                {   unfold keys_minus_p.
+                    (* In (token_pooled p) (FMap.keys (stor_rates prev_state)) *)
+                    pose proof (pool_entrypoint_check_2_pf prev_state new_state chain ctx p new_acts receive_some) as rate_exists.
+                    destruct rate_exists as [r_x rate_exists_el].
+                    apply FMap.In_elements in rate_exists_el.
+                    pose proof (in_map fst
+                        (FMap.elements (stor_rates prev_state))
+                        (token_pooled p, r_x)
+                        rate_exists_el)
+                    as rate_exists_key. clear rate_exists_el.
+                    simpl in rate_exists_key.
+                    (* recall NoDup keys *)
+                    pose proof (FMap.NoDup_keys (stor_rates prev_state))
+                    as nodup_keys.
+                    (* since NoDup keys, you can permute *)
+                    exact (nodup_permute 
+                        (token_pooled p) 
+                        (FMap.keys (stor_rates prev_state))
+                        token_eq_dec
+                        nodup_keys 
+                        rate_exists_key). }
+                (* Use the permutation to rewrite the LHS first, extracting (token_pooled p) *)
+                pose proof 
+                    (Permutation_map tokens_to_values_new)
+                        (* list 1 *)
+                        (FMap.keys (stor_rates prev_state))
+                        (* list 2 *)
+                        ((token_pooled p) :: keys_minus_p) 
+                        (* the previous permutation *)
+                        keys_permuted
+                as lhs_permute_map.
+                (* now that we have that permutation, rewrite in the suml *)
+                rewrite (suml_permute_commutes 
+                    (map tokens_to_values_new (FMap.keys (stor_rates prev_state)))
+                    (map tokens_to_values_new (token_pooled p :: keys_minus_p))
+                    lhs_permute_map).
+                (* now extract (token_pooled p) *)
+                rewrite (map_extract
+                    (token_pooled p)
+                    keys_minus_p
+                    tokens_to_values_new).
+                rewrite (suml_extract (tokens_to_values_new (token_pooled p))).
+                (* Now separate the sum on the RHS *)
+                pose proof 
+                    (Permutation_map tokens_to_values_prev)
+                        (* list 1 *)
+                        (FMap.keys (stor_rates prev_state))
+                        (* list 2 *)
+                        ((token_pooled p) :: keys_minus_p)
+                        (* the previous permutation *)
+                        keys_permuted
+                as rhs_permute_map.
+                (* now that we have that permutation, rewrite in the suml *)
+                rewrite (suml_permute_commutes 
+                    (map tokens_to_values_prev (FMap.keys (stor_rates prev_state)))
+                    (map tokens_to_values_prev (token_pooled p :: keys_minus_p))
+                    rhs_permute_map).
+                (* now extract (token_pooled p) *)
+                rewrite (map_extract
+                    (token_pooled p)
+                    keys_minus_p
+                    tokens_to_values_prev).
+                rewrite (suml_extract (tokens_to_values_prev (token_pooled p))).
+
+                (* Now proceed in two parts *)
+                (* first the sum of all the unchanged keys *)
+                assert 
+                    (suml (map tokens_to_values_new keys_minus_p) = 
+                     suml (map tokens_to_values_prev keys_minus_p))
+                as old_keys_eq.
+                {   assert (forall t, In t keys_minus_p -> t <> (token_pooled p))
+                    as t_neq.
+                    {   intros * H_in.
+                        unfold keys_minus_p in H_in.
+                        apply in_remove in H_in.
+                        destruct H_in as [_ res].
+                        exact res. }
+                    assert (forall t, In t keys_minus_p -> 
+                        tokens_to_values_new t = tokens_to_values_prev t)
+                    as tokens_to_vals_eq.
+                    {   intros * H_in.
+                        apply t_neq in H_in.
+                        apply bals_unchanged in H_in.
+                        unfold tokens_to_values_new, tokens_to_values_prev.
+                        rewrite H_in.
+                        reflexivity. }
+                    rewrite (mapped_eq
+                        token N
+                        tokens_to_values_new
+                        tokens_to_values_prev
+                        keys_minus_p
+                        tokens_to_vals_eq).
+                    reflexivity. }
+
+                (* then to the key that did change *)
+                assert
+                    (tokens_to_values_new (token_pooled p) = 
+                    tokens_to_values_prev (token_pooled p) + 
+                    get_rate (token_pooled p) (stor_rates prev_state) / 1000000 * qty_pooled p)
+                as new_key_eq.
+                {   unfold tokens_to_values_new, tokens_to_values_prev.
+                    (* get the calculation from the specification *)
+                    rewrite bal_update.
+                    (* rewrite some terms to simplify *)
+                    set (t := (token_pooled p)).
+                    set (rates := (stor_rates prev_state)).
+                    set (t_bal := get_bal t (stor_tokens_held prev_state)).
+                    set (q_pooled := qty_pooled p).
+                    set (rate_t := get_rate t rates).
+                    (* some simple algebraic manipulation *)
+                    rewrite (N.mul_add_distr_l).
+                    (* !!! TODO this is an inherent problem with the function definitions *)
+                        (* TODO this should be abstracted to the specification *)
+                        assert ((rate_t * t_bal + rate_t * q_pooled) / 1000000 = (rate_t * t_bal / 1000000 + rate_t * q_pooled / 1000000)) as div_distr. admit.
+                        rewrite div_distr. clear div_distr.
+                        (* TODO THIS TOO *)
+                        assert (rate_t / 1000000 * q_pooled = rate_t * q_pooled / 1000000) as div_comm. admit.
+                        rewrite div_comm. clear div_comm.
+                    (* END problem with function definitions *)
+                    reflexivity. }
+                rewrite old_keys_eq. rewrite new_key_eq.
+                rewrite <- N.add_assoc.
+                rewrite (N.add_comm
+                    (get_rate (token_pooled p) (stor_rates prev_state) / 1000000 * qty_pooled p)
+                    (suml (map tokens_to_values_prev keys_minus_p))).
+                rewrite N.add_assoc.
+                reflexivity. }
+            rewrite separate_sum. clear separate_sum.
+            rewrite out_update.
+            rewrite IH.
+            reflexivity.
+        (* m = unpool *)
+        +   is_sp_destruct.
+            (* understand how tokens_held has changed *)
+            pose proof (unpool_decreases_tokens_held_pf prev_state chain ctx u new_state new_acts
+                receive_some) as bal_update.
+            destruct bal_update as [bal_update bals_unchanged].
+            (* show all rates are the same *)
+            pose proof (unpool_rates_unchanged_pf prev_state new_state chain ctx u new_acts
+                receive_some) as rates_update.
+            (* show how the outstanding tokens update *)
+            pose proof (unpool_outstanding_pf prev_state new_state chain ctx u new_acts 
+                receive_some) as out_update.
+            simpl in out_update.
+            rewrite out_update. clear out_update.
+            (* because the rates are unchanged, summing over them is unchanged *)
+            assert (tokens_to_values (stor_rates new_state)  (stor_tokens_held new_state) = 
+                    tokens_to_values (stor_rates prev_state) (stor_tokens_held new_state))
+            as rates_unchanged.
+            {   unfold tokens_to_values.
+                rewrite (token_keys_invariant_unpool u new_state new_acts prev_state ctx chain receive_some).
+                apply map_ext.
+                intro t.
+                unfold get_rate. rewrite rates_update.
+                auto.  }
+            rewrite rates_unchanged. clear rates_unchanged.
+            (* now separate the sum *)
+            assert (suml (tokens_to_values (stor_rates prev_state) (stor_tokens_held new_state)) = 
+                    suml (tokens_to_values (stor_rates prev_state) (stor_tokens_held prev_state)) - 
+                        qty_unpooled u)
+            as separate_sum.
+            {   unfold tokens_to_values.
+                (* some simplifying notation *)
+                set (keys_minus_u := (remove token_eq_dec (token_unpooled u) (FMap.keys (stor_rates prev_state)))).
+                set (tokens_to_values_new := fun k : token => get_rate k (stor_rates prev_state) * get_bal k (stor_tokens_held new_state) / 1000000).
+                set (tokens_to_values_prev := fun k : token => get_rate k (stor_rates prev_state) * get_bal k (stor_tokens_held prev_state) / 1000000).
+                (* 1. show there's a Permutation with (token_pooled p) at the front *)
+                assert (Permutation
+                    (FMap.keys (stor_rates prev_state)) 
+                    ((token_unpooled u) :: keys_minus_u))
+                as keys_permuted.
+                {   unfold keys_minus_u.
+                    (* In (token_pooled p) (FMap.keys (stor_rates prev_state)) *)
+                    pose proof (unpool_entrypoint_check_2_pf prev_state new_state chain ctx u new_acts receive_some) as rate_exists.
+                    destruct rate_exists as [r_x rate_exists_el].
+                    apply FMap.In_elements in rate_exists_el.
+                    pose proof (in_map fst
+                        (FMap.elements (stor_rates prev_state))
+                        (token_unpooled u, r_x)
+                        rate_exists_el)
+                    as rate_exists_key. clear rate_exists_el.
+                    simpl in rate_exists_key.
+                    (* recall NoDup keys *)
+                    pose proof (FMap.NoDup_keys (stor_rates prev_state))
+                    as nodup_keys.
+                    (* since NoDup keys, you can permute *)
+                    exact (nodup_permute 
+                        (token_unpooled u) 
+                        (FMap.keys (stor_rates prev_state))
+                        token_eq_dec
+                        nodup_keys 
+                        rate_exists_key). }
+                (* Use the permutation to rewrite the LHS first, extracting (token_pooled p) *)
+                pose proof 
+                    (Permutation_map tokens_to_values_new)
+                        (* list 1 *)
+                        (FMap.keys (stor_rates prev_state))
+                        (* list 2 *)
+                        ((token_unpooled u) :: keys_minus_u) 
+                        (* the previous permutation *)
+                        keys_permuted
+                as lhs_permute_map.
+                (* now that we have that permutation, rewrite in the suml *)
+                rewrite (suml_permute_commutes 
+                    (map tokens_to_values_new (FMap.keys (stor_rates prev_state)))
+                    (map tokens_to_values_new (token_unpooled u :: keys_minus_u))
+                    lhs_permute_map).
+                (* now extract (token_pooled p) *)
+                rewrite (map_extract
+                    (token_unpooled u)
+                    keys_minus_u
+                    tokens_to_values_new).
+                rewrite (suml_extract (tokens_to_values_new (token_unpooled u))).
+                (* Now separate the sum on the RHS *)
+                pose proof 
+                    (Permutation_map tokens_to_values_prev)
+                        (* list 1 *)
+                        (FMap.keys (stor_rates prev_state))
+                        (* list 2 *)
+                        ((token_unpooled u) :: keys_minus_u)
+                        (* the previous permutation *)
+                        keys_permuted
+                as rhs_permute_map.
+                (* now that we have that permutation, rewrite in the suml *)
+                rewrite (suml_permute_commutes 
+                    (map tokens_to_values_prev (FMap.keys (stor_rates prev_state)))
+                    (map tokens_to_values_prev (token_unpooled u :: keys_minus_u))
+                    rhs_permute_map).
+                (* now extract (token_pooled p) *)
+                rewrite (map_extract
+                    (token_unpooled u)
+                    keys_minus_u
+                    tokens_to_values_prev).
+                rewrite (suml_extract (tokens_to_values_prev (token_unpooled u))).
+
+                (* Now proceed in two parts *)
+                (* first the sum of all the unchanged keys *)
+                assert 
+                    (suml (map tokens_to_values_new keys_minus_u) = 
+                     suml (map tokens_to_values_prev keys_minus_u))
+                as old_keys_eq.
+                {   assert (forall t, In t keys_minus_u -> t <> (token_unpooled u))
+                    as t_neq.
+                    {   intros * H_in.
+                        unfold keys_minus_u in H_in.
+                        apply in_remove in H_in.
+                        destruct H_in as [_ res].
+                        exact res. }
+                    assert (forall t, In t keys_minus_u -> 
+                        tokens_to_values_new t = tokens_to_values_prev t)
+                    as tokens_to_vals_eq.
+                    {   intros * H_in.
+                        apply t_neq in H_in.
+                        apply bals_unchanged in H_in.
+                        unfold tokens_to_values_new, tokens_to_values_prev.
+                        rewrite H_in.
+                        reflexivity. }
+                    rewrite (mapped_eq
+                        token N
+                        tokens_to_values_new
+                        tokens_to_values_prev
+                        keys_minus_u
+                        tokens_to_vals_eq).
+                    reflexivity. }
+                rewrite old_keys_eq. clear old_keys_eq.
+
+                (* then to the key that did change *)
+                assert
+                    (tokens_to_values_new (token_unpooled u) = 
+                    tokens_to_values_prev (token_unpooled u) - qty_unpooled u)
+                as new_key_eq.
+                {   unfold tokens_to_values_new, tokens_to_values_prev.
+                    (* get the calculation from the specification *)
+                    rewrite bal_update.
+                    (* rewrite some terms to simplify *)
+                    set (t := (token_unpooled u)).
+                    set (rates := (stor_rates prev_state)).
+                    set (t_bal_old := get_bal t (stor_tokens_held prev_state)).
+                    set (q_unpooled := qty_unpooled u).
+                    set (rate_t := get_rate t rates).
+                    (* some simple algebraic manipulation *)
+                    rewrite (N.mul_sub_distr_l t_bal_old (q_unpooled * 1_000_000 / rate_t) rate_t).
+                    assert ((rate_t * t_bal_old - rate_t * (q_unpooled * 1000000 / rate_t)) / 1000000 = 
+                    rate_t * t_bal_old / 1000000 - rate_t * (q_unpooled * 1000000 / rate_t) / 1000000)
+                    as div_distr. { admit. }
+                    rewrite div_distr. clear div_distr.
+                    assert (rate_t * (q_unpooled * 1000000 / rate_t) / 1000000 = q_unpooled) 
+                    as div_cancelled. { admit. } 
+                    rewrite div_cancelled. clear div_cancelled.
+                    reflexivity. }
+                rewrite new_key_eq.
+                
+                (* this is an additional condition required here so that commutativity applies *)
+                assert (qty_unpooled u <= tokens_to_values_prev (token_unpooled u))
+                as unpooled_leq. {
+                    unfold tokens_to_values_prev.
+                    exact (unpool_entrypoint_check_3_pf prev_state new_state chain ctx u new_acts receive_some). }
+                rewrite (N.add_sub_swap 
+                    (tokens_to_values_prev (token_unpooled u))
+                    (suml (map tokens_to_values_prev keys_minus_u))
+                    (qty_unpooled u)
+                    unpooled_leq).
+                reflexivity. }
+            rewrite separate_sum. clear separate_sum.
+            rewrite IH.
+            reflexivity.
+        (* m = trade *)
+        +   is_sp_destruct. clear is_sp.
+            (* understand how tokens_held has changed *)
+            pose proof (trade_tokens_held_update_pf prev_state chain ctx t new_state new_acts 
+                receive_some) as tokens_held_update.
+            destruct tokens_held_update as [tokens_held_update_ty tokens_held_update].
+            destruct tokens_held_update as [tokens_held_update_tx tokens_held_update_tz].
+            (* how calling trade updates rates *)
+            pose proof (trade_update_rates_formula_pf prev_state chain ctx t new_state new_acts
+                receive_some) as rates_changed_and_unchanged.
+            destruct rates_changed_and_unchanged as [tx_neq_ty rates_changed_and_unchanged].
+            destruct rates_changed_and_unchanged as [rx_change rz_unchanged].
+            (* how outstanding_tokens has changed by calling trade *)
+            pose proof (trade_outstanding_update_pf prev_state chain ctx t new_state new_acts 
+                receive_some) as out_update.
+            rewrite out_update. clear out_update.
+            (* LHS equals sum over tokens except for tx and ty, plus r_x' * etc , minus r_y * delta_y *)
+
+            (* LHS *)
+            (* permute FMap.keys (stor_tokens_held new_state) to have tx :: ty :: keys' *)
+                (* for these, rates and balances are all the same as before *)
+            
+            (* separate LHS into ^^, plus new rate * t_x, minus rate * t_y *)
+
+            (* permute FMap.keys for the OLD suml to MANIPULATE the inductive hypothesis IH *)
+
+            (* then assert NEW decomposed suml = OLD decomposed suml
+                <=> new_rate * t_x - rate * t_y = old_rate * t_x - rate * t_y (something like that) *)
+                (* ** will require additional assumptions on rate, etc. ** *)
+
+            (* rewrite that assertion; prove by IH *)
+
+            admit. (* TODO algebra *)
     (* Please reestablish the invariant after a recursive call *)
-    -   admit. (* probably the same proof *)
+    -   admit. (* TODO probably the same proof *)
     (* solve remaining facts *)
     -   solve_facts.
 Admitted.
